got init proof working: fixed three bugs in spec + interp; refactored a defn for easier provin'

tla-tree/CrashableMap.dfy
@@ -17,15 +17,20 @@ datatype Variables = Variables(views:seq<View>)
 // give; we may well need to relax it later to allow the implementation more
 // freedom.)
 
-predicate completeMap(a:imap<Key,Value>)
+predicate ViewComplete(view:View)
 {
-    forall k :: k in a
+    forall k :: k in view
+}
+
+predicate AllViewsComplete(views:seq<View>)
+{
+    forall i :: 0<=i<|views| ==> ViewComplete(views[i])
 }
 
 predicate WF(s:Variables)
 {
     && 0 < |s.views|
-    && forall i :: 0<=i<|s.views| ==> completeMap(s.views[i])
+    && AllViewsComplete(s.views)
 }
 
 // Dafny black magic: This name is here to give EmptyMap's forall something to
@@ -36,7 +41,7 @@ predicate InDomain(k:Key)
 }
 
 function EmptyMap() : (zmap : imap<Key,Value>)
-    ensures completeMap(zmap)
+    ensures ViewComplete(zmap)
 {
     imap k | InDomain(k) :: EmptyValue()
 }
@@ -53,6 +58,12 @@ function EphemeralView(k:Constants, s:Variables) : View
     s.views[0]
 }
 
+function PersistentView(k:Constants, s:Variables) : View
+    requires WF(s)
+{
+    s.views[|s.views|-1]
+}
+
 predicate Query(k:Constants, s:Variables, s':Variables, datum:Datum)
     requires WF(s)
 {
@@ -62,11 +73,19 @@ predicate Query(k:Constants, s:Variables, s':Variables, datum:Datum)
 
 predicate Write(k:Constants, s:Variables, s':Variables, datum:Datum)
     requires WF(s)
+    ensures Write(k, s, s', datum) ==> WF(s')
 {
-    // Prepend a new ephemeral view. Prior view remains on the view
-    // stack that's allowed to appear after a crash.
-    var newView := EphemeralView(k, s)[datum.key := datum.value];
-    s'.views == [newView] + s.views
+    // Prepend a new ephemeral view, and preserve the committed persistent view.
+    && WF(s')
+    && EphemeralView(k, s') == EphemeralView(k, s)[datum.key := datum.value]
+    && PersistentView(k, s') == PersistentView(k, s)
+
+    // You're allowed to drop intermediate views, but if you keep them, they
+    // need to maintain the order from earlier writes. (This is all or nothing:
+    // keep them all if you're the log, keep nothing if you're the tree. One
+    // could imagine allowing selective drop of intermediate views, but we
+    // don't need it, so we didn't write it.)
+    && (2 < |s'.views| ==> s'.views[1..] == s.views)
 }
 
 // Report to the user that the disk is synchronized with the memory.
@@ -100,18 +119,24 @@ predicate Stutter(k:Constants, s:Variables, s':Variables)
     s' == s
 }
 
-datatype Step = Query(datum:Datum) | WriteStep(datum:Datum) | CompleteSync | PersistWritesStep(writesRetired:int) | SpontaneousCrashStep | Stutter
+datatype Step =
+    | QueryStep(datum:Datum)
+    | WriteStep(datum:Datum)
+    | CompleteSyncStep
+    | PersistWritesStep(writesRetired:int)
+    | SpontaneousCrashStep
+    | StutterStep
 
 predicate NextStep(k:Constants, s:Variables, s':Variables, step:Step)
     requires WF(s)
 {
-    match step {
-        case Query(datum) => Query(k, s, s', datum)
+    && match step {
+        case QueryStep(datum) => Query(k, s, s', datum)
         case WriteStep(datum) => Write(k, s, s', datum)
-        case CompleteSync() => CompleteSync(k, s, s')
+        case CompleteSyncStep() => CompleteSync(k, s, s')
         case PersistWritesStep(writesRetired) => PersistWrites(k, s, s', writesRetired)
         case SpontaneousCrashStep() => SpontaneousCrash(k, s, s')
-        case Stutter() => Stutter(k, s, s')
+        case StutterStep() => Stutter(k, s, s')
     }
 }
 
