tla-tree/ImmutableDiskTreeRefinement.dfy
@@ -2,11 +2,13 @@ include "CrashableMap.dfy"
 include "ImmutableDiskTreeInterpretation.dfy"
 
 module ImmutableDiskTreeRefinement {
+import opened KVTypes
 import opened TreeTypes
 import opened ImmutableDiskTree
 import opened ImmutableDiskTreeInv
 import opened ImmutableDiskTreeHeight
 import opened ImmutableDiskTreeInterpretation
+import opened MissingLibrary
 import CrashableMap
 
 lemma InvImpliesRefinementInit(k:Constants, s:Variables)
@@ -14,7 +16,21 @@ lemma InvImpliesRefinementInit(k:Constants, s:Variables)
     requires TreeInv(k, s)
     ensures CrashableMap.Init(Ik(k), I(k, s))
 {
+    reveal_ISubtreePrefixView();
+    reveal_ISlotView();
+    var tv := PersistentTreeView(k, s);
+    assert ISubtreeView(tv, ROOT_ADDR()) == ISubtreePrefixView(tv, ROOT_ADDR(), /*slotCount*/ 1); // OBSERVE
+    assert IPersistentView(k, s) == CrashableMap.EmptyMap(); // OBSERVE
 } 
+
+function FetchStep(k:Constants, s:Variables, s':Variables) : (step:Step)
+    requires Next(k, s, s')
+    ensures NextStep(k, s, s', step)
+{
+    reveal_Next();
+    var step :| NextStep(k, s, s', step);
+    step
+}
 
 lemma InvImpliesRefinementNext(k:Constants, s:Variables, s':Variables)
     requires Next(k, s, s')
@@ -24,6 +40,49 @@ lemma InvImpliesRefinementNext(k:Constants, s:Variables, s':Variables)
     ensures CrashableMap.WF(I(k, s'))
     ensures CrashableMap.Next(Ik(k), I(k, s), I(k, s'))
 {
+    var Ik := Ik(k);
+    var Is := I(k, s);
+    var Is' := I(k, s');
+    var step := FetchStep(k, s, s');
+
+    match step {
+        case QueryActionStep(lookup, datum) => {
+            assert CrashableMap.Query(Ik, Is, Is', datum);
+        }
+        case InsertActionStep(edit, datum) => {
+            assert CrashableMap.Write(Ik, Is, Is', datum);
+        }
+        case DeleteActionStep(edit, datum) => {
+            assert CrashableMap.Write(Ik, Is, Is', Datum(datum.key, EmptyValue()));
+        }
+        case ExpandActionStep(j) => {
+            assert CrashableMap.Stutter(Ik, Is, Is');
+        }
+        case ContractActionStep(j) => {
+            assert CrashableMap.Stutter(Ik, Is, Is');
+        }
+        case WriteBackActionStep(lba) => {
+            assert CrashableMap.Stutter(Ik, Is, Is');
+        }
+        case EmitTableActionStep(persistentTi, super, tblSectorIdx) => {
+            assert CrashableMap.Stutter(Ik, Is, Is');
+        }
+        case CommitActionStep(persistentTi, super) => {
+            assert CrashableMap.PersistWrites(Ik, Is, Is', 1);
+        }
+        case CrashActionStep => {
+            assert CrashableMap.SpontaneousCrash(Ik, Is, Is');
+        }
+        case RecoverActionStep(super, persistentTl) => {
+            assert CrashableMap.Stutter(Ik, Is, Is');
+        }
+        case CacheFaultActionStep(lba, sector) => {
+            assert CrashableMap.Stutter(Ik, Is, Is');
+        }
+        case CacheEvictActionStep(lba) => {
+            assert CrashableMap.Stutter(Ik, Is, Is');
+        }
+    }
 }
 
 } // module ImmutableDiskTreeRefinement
