tla-tree/MissingLibrary.dfy
@@ -6,10 +6,18 @@ function Last<T>(s:seq<T>) : T  // TODO move to library
     s[|s|-1]
 }
 
-function {:opaque} EmptyMap<K(!new),V>(any:V) : (e:map<K,V>)
+function {:opaque} EmptyImap<K(!new),V>() : (e:imap<K,V>)
+    ensures e.Keys == iset{}
+{
+    var v :| true;
+    imap k | k in {} :: v
+}
+
+function {:opaque} EmptyMap<K(!new),V>() : (e:map<K,V>)
     ensures e.Keys == {}
 {
-    map k | k in {} :: any
+    var v :| true;
+    map k | k in {} :: v
 }
 
 function {:opaque} MapRemove<K,V>(m:map<K,V>, k:K) : (m':map<K,V>)
